transformations/Moore2Mealy/theorems/WFStable.v
@@ -19,12 +19,11 @@ Import Model Semantics.
 
 Lemma WF_transition_source_uniqueness_stable :
   forall m,
-    Moore.WF_transition_target_exists m ->
     Moore.WF_transition_source_exists m -> 
     MooreWF.WF_transition_source_uniqueness m -> 
     MealyWF.WF_transition_source_uniqueness (Semantics.execute Moore2Mealy.Moore2Mealy m).
 Proof.
-  intros m WF1 WF2 WF4.
+  intros m  WF2 WF4.
   unfold MealyWF.WF_transition_source_uniqueness.
   intros. 
 
@@ -33,8 +32,8 @@ Proof.
   simpl in H1. subst t''.
   f_equal.
   
-  destruct (Links.source_link_bw _ WF1 WF2 _ _ H) as (s1 & C1 & IN1).
-  destruct (Links.source_link_bw _ WF1 WF2 _ _ H0) as (s2 & C2 & IN2).
+  destruct (Links.source_link_bw _ WF2 _ _ H) as (s1 & C1 & IN1).
+  destruct (Links.source_link_bw _ WF2 _ _ H0) as (s2 & C2 & IN2).
 
   specialize (WF4 _ _ IN1 IN2 (eq_refl _)). 
   PropUtils.inj WF4.
